#### Natural log is defined as 

$$
ln(x) = \int_{1}^{x}\frac{1}{t} dt
$$
### Hence, we deduce that  
$$
\begin{align*}
ln(1) = 0  \\
ln(ax) = ln(x) + ln(a)
\end{align*}
$$
Proof
1. let a be an constant and x be an variable
$$
\begin{align*}
\frac{d}{dx}(ln(ax)) &= \frac{a}{ax} = \frac{1}{x} = \frac{d}{dx}(ln(x)) \\
\Leftrightarrow ln(ax) &= ln(x) + c \\
\end{align*}
$$
Subs  x = 1
$$
\begin{align*}
c &= ln(a) \\
ln(ax) &= ln(x) + ln(a)
\end{align*}
$$
$$
\begin{align*}
ln: \mathbb{R} \rightarrow (0, \infty) \\
exp: (0, \infty) \rightarrow \mathbb{R}
\end{align*}
$$
$exp$ is defined as inverse of $ln$
